Ed: Proof of Load

code/experimental/ed25519/Hacl.Impl.Load56.fst
@@ -10,6 +10,9 @@ open Lib.Buffer
 open Lib.ByteBuffer
 
 module F56 = Hacl.Impl.Ed25519.Field56
+module S56 = Hacl.Spec.Ed25519.Field56.Definition
+
+#reset-options "--z3rlimit 20 --max_fuel 0 --max_ifuel 0"
 
 val hload56_le:
     b:lbuffer uint8 64ul
@@ -48,12 +51,79 @@ val hload56_le':
   -> off:size_t{v off <= 21} ->
   Stack uint64
     (requires fun h -> live h b)
-    (ensures fun h0 z h1 -> h0 == h1)
+    (ensures fun h0 z h1 -> h0 == h1 /\
+      v z < 0x100000000000000 /\
+      v z == nat_from_bytes_le (Seq.slice (as_seq h0 b) (v off) (v off + 7))
+    )
+
+#push-options "--z3rlimit 50"
+
 let hload56_le' b off =
+  let h0 = get() in
   let b8 = sub b off 8ul in
   let z  = uint_from_bytes_le b8 in
   let z' = z &. u64 0xffffffffffffff in
+  assert_norm (0xffffffffffffff == pow2 56 - 1);
+  assert_norm (0x100000000000000 == pow2 56 );
+  calc (==) {
+    v z' <: nat;
+    (==) { }
+    v (z &. u64 0xffffffffffffff);
+    (==) { logand_spec z (u64 0xffffffffffffff) }
+    v z `logand_v` 0xffffffffffffff;
+    (==) { assert_norm(pow2 56 - 1 == 0xffffffffffffff); UInt.logand_mask (UInt.to_uint_t 64 (v z)) 56 }
+    (v z % pow2 56);
+    (==) { lemma_reveal_uint_to_bytes_le #U64 #SEC (as_seq h0 b8) }
+    nat_from_bytes_le (as_seq h0 b8) % pow2 56;
+    (==) { nat_from_intseq_le_slice_lemma (as_seq h0 b8) 7 }
+    (nat_from_bytes_le (Seq.slice (as_seq h0 b8) 0 7) +
+      pow2 (7 * 8) * nat_from_bytes_le (Seq.slice (as_seq h0 b8) 7 8)) % pow2 56;
+    (==) { FStar.Math.Lemmas.lemma_mod_plus_distr_r
+      (nat_from_bytes_le (Seq.slice (as_seq h0 b8) 0 7))
+      (pow2 (7 * 8) * nat_from_bytes_le (Seq.slice (as_seq h0 b8) 7 8))
+      (pow2 56);
+      FStar.Math.Lemmas.swap_mul (pow2 (7 * 8)) (nat_from_bytes_le (Seq.slice (as_seq h0 b8) 7 8));
+        FStar.Math.Lemmas.cancel_mul_mod (nat_from_bytes_le (Seq.slice (as_seq h0 b8) 7 8)) (pow2 56) }
+    nat_from_bytes_le (Seq.slice (as_seq h0 b8) 0 7) <: nat;
+  };
+  assert (Seq.equal
+        (Seq.slice (as_seq h0 b) (v off) (v off + 7))
+        (Seq.slice (as_seq h0 b8) 0 7));
   z'
+
+#pop-options
+
+let lemma_nat_from_bytes_le_append (k1 k2:bytes) : Lemma
+  (requires Seq.length k1 + Seq.length k2 <= max_size_t)
+  (ensures nat_from_bytes_le (Seq.append k1 k2) ==
+  nat_from_bytes_le k1 + pow2 (Seq.length k1 * 8) * nat_from_bytes_le k2) =
+  let k = Seq.append k1 k2 in
+  let n = Seq.length k1 + Seq.length k2 in
+  nat_from_intseq_le_slice_lemma #U8 #SEC #n k (Seq.length k1);
+  assert (k1 `Seq.equal` Seq.slice k 0 (Seq.length k1));
+  assert (k2 `Seq.equal` Seq.slice k (Seq.length k1) n)
+
+let lemma_load_32_bytes (k:lbytes 32) (b0 b1 b2 b3 b4:uint64) : Lemma
+  (requires
+    v b0 == nat_from_bytes_le (Seq.slice k 0 7) /\
+    v b1 == nat_from_bytes_le (Seq.slice k 7 14) /\
+    v b2 == nat_from_bytes_le (Seq.slice k 14 21) /\
+    v b3 == nat_from_bytes_le (Seq.slice k 21 28) /\
+    v b4 == nat_from_bytes_le (Seq.slice k 28 32))
+  (ensures S56.as_nat5 (b0, b1, b2, b3, b4) == nat_from_bytes_le k)
+  =
+  lemma_nat_from_bytes_le_append (Seq.slice k 0 7) (Seq.slice k 7 14);
+  lemma_nat_from_bytes_le_append (Seq.slice k 0 14) (Seq.slice k 14 21);
+  lemma_nat_from_bytes_le_append (Seq.slice k 0 21) (Seq.slice k 21 28);
+  lemma_nat_from_bytes_le_append (Seq.slice k 0 28) (Seq.slice k 28 32);
+  assert (Seq.append (Seq.slice k 0 7) (Seq.slice k 7 14) `Seq.equal` Seq.slice k 0 14);
+  assert (Seq.append (Seq.slice k 0 14) (Seq.slice k 14 21) `Seq.equal` Seq.slice k 0 21);
+  assert (Seq.append (Seq.slice k 0 21) (Seq.slice k 21 28) `Seq.equal` Seq.slice k 0 28);
+  assert (Seq.append (Seq.slice k 0 28) (Seq.slice k 28 32) `Seq.equal` k);
+  assert_norm (pow2 56 == 0x100000000000000);
+  assert_norm (pow2 112 == 0x10000000000000000000000000000);
+  assert_norm (pow2 168 == 0x1000000000000000000000000000000000000000000);
+  assert_norm (pow2 224 == 0x100000000000000000000000000000000000000000000000000000000)
 
 val load_32_bytes:
   out:lbuffer uint64 5ul
@@ -70,12 +140,15 @@ val load_32_bytes:
        v s.[3] < 0x100000000000000 /\
        v s.[4] < 0x100000000000000)
     )
+
 let load_32_bytes out b =
+  let h0 = get() in
   let b0 = hload56_le' b 0ul in
   let b1 = hload56_le' b 7ul in
   let b2 = hload56_le' b 14ul in
   let b3 = hload56_le' b 21ul in
   let b4 = uint_from_bytes_le #U32 (sub b 28ul 4ul) in
   let b4 = to_u64 b4 in
-  admit();
+  lemma_reveal_uint_to_bytes_le #U32 (as_seq h0 (gsub b 28ul 4ul));
+  lemma_load_32_bytes (as_seq h0 b) b0 b1 b2 b3 b4;
   Hacl.Bignum25519.make_u64_5 out b0 b1 b2 b3 b4
